cfrontend/BeePL_typesystem.v
@@ -2,21 +2,23 @@ Require Import String ZArith Coq.FSets.FMapAVL Coq.Structures.OrderedTypeEx.
 Require Import Coq.FSets.FSetProperties Coq.FSets.FMapFacts FMaps FSetAVL Nat PeanoNat.
 Require Import Coq.Arith.EqNat Coq.ZArith.Int Integers AST Maps.
 Require Import BeePL_aux BeePL_mem BeeTypes BeePL.
+From mathcomp Require Import all_ssreflect. 
 
 Definition empty_effect : effect := nil. 
 
 Inductive type_expr : ty_context -> store_context -> expr -> effect -> type -> Prop :=
 | Ty_var : forall Gamma Sigma x t, 
-           get_ty Gamma x = Some t ->
-           type_expr Gamma Sigma (Var x t) empty_effect t
+           get_ty Gamma x.(vname) = Some t ->
+           x.(vtype) = t ->
+           type_expr Gamma Sigma (Var x) empty_effect t
 | Ty_const : forall Gamma Sigma c t,
-             type_expr Gamma Sigma c empty_effect t
+             type_expr Gamma Sigma (Const c t) empty_effect t
 | Ty_appr : forall Gamma Sigma r e es h bt rt ef efs ts, 
-            get_ty Gamma r = Some rt ->
-            type_expr Gamma Sigma (Var r rt) empty_effect rt -> 
+            get_ty Gamma r.(vname) = Some rt ->
+            type_expr Gamma Sigma (Var r) empty_effect rt -> 
             type_expr Gamma Sigma e ef (Reftype h bt) -> 
             type_exprs Gamma Sigma es efs ts -> 
-            type_expr Gamma Sigma (App (Some r) e es rt) (ef ++ efs) rt
+            type_expr Gamma Sigma (App (Some r.(vname)) e es rt) (ef ++ efs) rt
 | Ty_app : forall Gamma Sigma e es h bt rt ef ts, 
            type_expr Gamma Sigma e ef (Reftype h bt) -> 
            type_exprs Gamma Sigma es ef ts -> 
@@ -48,8 +50,8 @@ Inductive type_expr : ty_context -> store_context -> expr -> effect -> type -> P
             type_expr Gamma Sigma e3 ef' t ->
             type_expr Gamma Sigma (Cond e1 e2 e3 t) (ef ++ ef') t
 | Ty_loc : forall Gamma Sigma l h bt,
-           get_sty Sigma l = Some bt ->
-           type_expr Gamma Sigma (Addr l bt) empty_effect (Reftype h bt) 
+           get_sty Sigma l.(lname) = Some bt ->
+           type_expr Gamma Sigma (Addr l) empty_effect (Reftype h bt) 
 with type_exprs : ty_context -> store_context -> list expr -> effect -> list type -> Prop :=
 | Ty_nil : forall Gamma Sigma,
            type_exprs Gamma Sigma nil nil nil
@@ -59,3 +61,58 @@ with type_exprs : ty_context -> store_context -> list expr -> effect -> list typ
             type_exprs Gamma Sigma (e :: es) (ef ++ efs) (t :: ts).
            
 
+(**** Supoorting lemmas ****)
+Lemma get_ty_write_var : forall Gamma vm r v vm' t,
+write_var vm r v = vm' ->
+typeof_value v t ->
+get_ty Gamma r.(vname) = Some t.
+Proof.
+Admitted.
+
+Lemma write_var_preserve_ty : forall Gamma Sigma vm r rv vm' t,
+write_var vm r rv = vm' ->
+typeof_value rv t ->
+type_expr Gamma Sigma (Var r) empty_effect t.
+Proof.
+Admitted.
+
+(**** Preservation ****)
+Lemma preservation : forall Gamma Sigma genv e ef t st st' v, 
+type_expr Gamma Sigma e ef t ->
+sem_expr genv st e st' v ->
+typeof_value v t.
+Proof.
+move=> Gamma Sigma genv e ef t st st' v ht he. move: st st' ef t ht he. elim: e=> //=.
+(* Var *)
++ admit.
+(* Const *)
++ move=> c t' st st' ef t /= ht /= he; inversion he; subst.
+  (* Int *)
+  + rewrite /typeof_value /=. case: t ht=> //= p.
+    + case: p=> //=.
+      + by move=> ht; inversion ht.
+      + by move=> ht; inversion ht.
+      + by move=> ht; inversion ht.
+    by move=> b ht; inversion ht.
+  by move=> e t ht;inversion ht.
+  (* Bool *)   
+  + rewrite /typeof_value /=. case: t ht=> //= p.
+    + case: p=> //=.
+      + by move=> ht; inversion ht.
+      + by move=> ht; inversion ht.
+      + by move=> ht; inversion ht.
+    by move=> b' ht;inversion ht.
+  by move=> e t ht;inversion ht.
+  (* Unit *)
+  + rewrite /typeof_value /=. case: t ht=> //= p.
+    + case: p=> //=.
+      + by move=> ht; inversion ht.
+      + by move=> ht; inversion ht.
+      + by move=> ht; inversion ht.
+    by move=> b' ht;inversion ht.
+  by move=> e t ht;inversion ht.
+(* App *)
++ move=> o e ih es ts st st' ef t ht he; inversion he; subst.
+  inversion ht; subst. admit.
+Admitted.
+  
